MutableMap.Realloc WIP

lib/MutableMap.dfy
@@ -11,7 +11,12 @@ module MutableMap {
 
   datatype Slot = Slot(slot: nat)
 
-  datatype Item<V(==)> = Empty | Filled(key: uint64, value: V) | Tombstone(key: uint64)
+  datatype Item<V(==)> = Empty | Entry(key: uint64, value: V) | Tombstone(key: uint64)
+
+  predicate ValidSlot(elementsLength: nat, slot: Slot)
+  {
+    slot.slot < elementsLength
+  }
 
   // FIXME(utaal) reduce proofs!
   class FixedSizeHashMap<V(==)> {
@@ -39,11 +44,6 @@ module MutableMap {
       reads this, this.Storage
     {
       key % (Storage.Length as uint64)
-    }
-
-    predicate ValidSlot(elementsLength: nat, slot: Slot)
-    {
-      slot.slot < elementsLength
     }
 
     function SlotSuccessor(elementsLength: nat, slot: Slot): (nextSlot: Slot)
@@ -96,7 +96,7 @@ module MutableMap {
       requires ValidSlot(|elements|, slot)
     {
       || (elements[slot.slot].Tombstone? && elements[slot.slot].key != excludingKey)
-      || (elements[slot.slot].Filled? && elements[slot.slot].key != excludingKey)
+      || (elements[slot.slot].Entry? && elements[slot.slot].key != excludingKey)
     }
 
     predicate FilledWithOtherKeys(elements: seq<Item<V>>, start: Slot, count: nat, excludingKey: uint64)
@@ -111,7 +111,7 @@ module MutableMap {
       requires ValidElements(elements)
       requires ValidSlot(|elements|, slot)
     {
-      (elements[slot.slot].Filled? || elements[slot.slot].Tombstone?) && elements[slot.slot].key == key
+      (elements[slot.slot].Entry? || elements[slot.slot].Tombstone?) && elements[slot.slot].key == key
     }
 
     predicate SlotExplainsKey(elements: seq<Item<V>>, skips: nat, key: uint64)
@@ -127,14 +127,14 @@ module MutableMap {
       requires ValidElements(elements)
     {
       && (forall key :: key in contents ==> exists skips :: SlotExplainsKey(elements, skips, key))
-      && (forall slot :: ValidSlot(|elements|, slot) && (elements[slot.slot].Filled? || elements[slot.slot].Tombstone?) ==>
+      && (forall slot :: ValidSlot(|elements|, slot) && (elements[slot.slot].Entry? || elements[slot.slot].Tombstone?) ==>
         && var key := elements[slot.slot].key;
         && key in contents)
       && (forall slot1, slot2 :: (
         && ValidSlot(|elements|, slot1)
         && ValidSlot(|elements|, slot2)
-        && (elements[slot1.slot].Filled? || elements[slot1.slot].Tombstone?)
-        && (elements[slot2.slot].Filled? || elements[slot2.slot].Tombstone?)
+        && (elements[slot1.slot].Entry? || elements[slot1.slot].Tombstone?)
+        && (elements[slot2.slot].Entry? || elements[slot2.slot].Tombstone?)
         && elements[slot1.slot].key == elements[slot2.slot].key
       ) ==> slot1 == slot2)
     }
@@ -148,7 +148,7 @@ module MutableMap {
 
       && |Contents| == (Count as nat)
       && SeqMatchesContentKeys(Storage[..], Contents)
-      && (forall slot :: ValidSlot(Storage.Length, slot) && Storage[slot.slot].Filled? ==>
+      && (forall slot :: ValidSlot(Storage.Length, slot) && Storage[slot.slot].Entry? ==>
           && var item := Storage[slot.slot];
           && Contents[item.key] == Some(item.value))
       && (forall slot :: ValidSlot(Storage.Length, slot) && Storage[slot.slot].Tombstone? ==>
@@ -159,7 +159,7 @@ module MutableMap {
     function IndexSetThrough(elements: seq<Item<V>>, through: nat): set<int>
       requires through <= |elements|
     {
-      set i | 0 <= i < through && (elements[i].Filled? || elements[i].Tombstone?)
+      set i | 0 <= i < through && (elements[i].Entry? || elements[i].Tombstone?)
     }
 
     function IndexSet(elements: seq<Item<V>>): set<int>
@@ -169,7 +169,7 @@ module MutableMap {
 
     function Count1(item: Item<V>): nat
     {
-      if item.Filled? || item.Tombstone? then 1 else 0
+      if item.Entry? || item.Tombstone? then 1 else 0
     }
 
     function CountFilled(view: seq<Item<V>>): (result: nat)
@@ -191,7 +191,7 @@ module MutableMap {
         var j := i + 1;
         CountFilledAdditive(elements[..i], [elements[i]]);
         assert elements[..i] + [elements[i]] == elements[..j];
-        if elements[i].Filled? || elements[i].Tombstone? {
+        if elements[i].Entry? || elements[i].Tombstone? {
           assert IndexSetThrough(elements, j) == IndexSetThrough(elements, i) + {i};
         } else {
           assert IndexSetThrough(elements, j) == IndexSetThrough(elements, i);
@@ -236,7 +236,9 @@ module MutableMap {
     constructor (size: uint64)
       requires 0 < size
       ensures Inv()
+      ensures forall slot :: ValidSlot(Storage.Length, slot) ==> Storage[slot.slot].Empty?
       ensures Contents == map[]
+      ensures fresh(Storage)
     {
       Count := 0;
       Storage := new [size] (_ => Empty);
@@ -295,7 +297,7 @@ module MutableMap {
       ensures slotIdx as nat == KthSlotSuccessor(Storage.Length, Slot(startSlotIdx as nat), ghostSkips as nat).slot
       ensures key in Contents ==> SlotExplainsKey(Storage[..], ghostSkips as nat, key)
       ensures key !in Contents ==> FilledWithOtherKeys(Storage[..], Slot(startSlotIdx as nat), ghostSkips as nat, key) && (Storage[slotIdx].Empty? || (Storage[slotIdx].Tombstone? && Storage[slotIdx].key == key))
-      ensures Storage[slotIdx].Filled? ==> key in Contents && key == Storage[slotIdx].key
+      ensures Storage[slotIdx].Entry? ==> key in Contents && key == Storage[slotIdx].key
       ensures Storage[slotIdx].Empty? ==> key !in Contents
     {
       slotIdx := Uint64SlotForKey(key);
@@ -347,7 +349,7 @@ module MutableMap {
         } else if Storage[slotIdx].key == key {
           return;
         }
-        assert Storage[slotIdx].Filled? || (Storage[slotIdx].Tombstone? && Storage[slotIdx].key != key);
+        assert Storage[slotIdx].Entry? || (Storage[slotIdx].Tombstone? && Storage[slotIdx].key != key);
         assert CountFilled(viewFromStartSlot[..skips]) == skips as nat;
         assert Storage[slotIdx] == viewFromStartSlot[skips];
         assert slotIdx as nat == KthSlotSuccessor(Storage.Length, startSlot, skips as nat).slot;
@@ -366,7 +368,7 @@ module MutableMap {
           assert Storage[slotIdx] == viewFromStartSlot[skips];
         }
         assert CountFilled(viewFromStartSlot[..skipsBefore]) == skipsBefore as nat;
-        assert viewFromStartSlot[skipsBefore].Filled? || viewFromStartSlot[skipsBefore].Tombstone?;
+        assert viewFromStartSlot[skipsBefore].Entry? || viewFromStartSlot[skipsBefore].Tombstone?;
         assert viewFromStartSlot[..skips] == viewFromStartSlot[..skipsBefore] + [viewFromStartSlot[skipsBefore]];
         assert CountFilled([viewFromStartSlot[skipsBefore]]) == 1;
         CountFilledAdditive(viewFromStartSlot[..skipsBefore], [viewFromStartSlot[skipsBefore]]);
@@ -398,7 +400,7 @@ module MutableMap {
       } else {
         assert key in Contents;
       }
-      Storage[slotIdx] := Filled(key, value);
+      Storage[slotIdx] := Entry(key, value);
       Contents := Contents[key := Some(value)];
       // --------------
 
@@ -424,8 +426,8 @@ module MutableMap {
       assert forall slot1, slot2 :: (
         && ValidSlot(Storage.Length, slot1)
         && ValidSlot(Storage.Length, slot2)
-        && Storage[slot1.slot].Filled?
-        && Storage[slot2.slot].Filled?
+        && Storage[slot1.slot].Entry?
+        && Storage[slot2.slot].Entry?
         && Storage[slot1.slot].key == Storage[slot2.slot].key
       ) ==> slot1 == slot2;
       assert Count as nat < Storage.Length;
@@ -439,7 +441,7 @@ module MutableMap {
     {
       var slotIdx, /* ghost */ probeStartSlotIdx, /* ghost */ probeSkips := Probe(key);
 
-      if Storage[slotIdx].Filled? {
+      if Storage[slotIdx].Entry? {
         assert key in Contents;
         found := Some(Storage[slotIdx].value);
         assert found == Contents[key];
@@ -466,7 +468,7 @@ module MutableMap {
     {
       var slotIdx, /* ghost */ probeStartSlotIdx, /* ghost */ probeSkips := Probe(key);
 
-      if Storage[slotIdx].Filled? {
+      if Storage[slotIdx].Entry? {
         assert key in Contents;
 
         // -- mutation --
@@ -494,6 +496,221 @@ module MutableMap {
         assert Inv();
       }
     }
+
+  }
+
+  class ResizingHashMap<V(==)> {
+    var Underlying: FixedSizeHashMap<V>;
+    var Count: uint64;
+
+    ghost var Contents: map<uint64, V>;
+
+    function MapFromStorage(elements: seq<Item<V>>): (result: map<uint64, V>)
+    {
+      if |elements| == 0 then
+        map[]
+      else
+        var item := Last(elements);
+        var dropLastMap := MapFromStorage(DropLast(elements));
+        if item.Entry? then
+          dropLastMap[item.key := item.value]
+        else
+          dropLastMap
+    }
+
+    lemma CantEquivocateMapFromStorageKey(underlying: FixedSizeHashMap<V>)
+      requires underlying.Inv()
+      ensures forall slot1, slot2 :: ValidSlot(underlying.Storage.Length, slot1) && ValidSlot(underlying.Storage.Length, slot2) &&
+          underlying.Storage[slot1.slot].Entry? && underlying.Storage[slot2.slot].Entry? &&
+          underlying.Storage[slot1.slot].key == underlying.Storage[slot2.slot].key ==> slot1 == slot2
+    {
+      assert underlying.Storage.Length > 0;
+      assert ValidSlot(underlying.Storage.Length, Slot(0));
+      assert exists slot :: ValidSlot(underlying.Storage.Length, slot);
+      var slot1 :| ValidSlot(underlying.Storage.Length, slot1);
+      var slot2 :| ValidSlot(underlying.Storage.Length, slot2);
+      if underlying.Storage[slot1.slot].Entry? && underlying.Storage[slot2.slot].Entry? &&
+        underlying.Storage[slot1.slot].key == underlying.Storage[slot2.slot].key {
+
+        if slot1 != slot2 {
+          assert false;
+        }
+      }
+    }
+
+    lemma MapFromStorageProperties(elements: seq<Item<V>>, result: map<uint64, V>)
+      requires forall slot1, slot2 :: ValidSlot(|elements|, slot1) && ValidSlot(|elements|, slot2) &&
+          elements[slot1.slot].Entry? && elements[slot2.slot].Entry? &&
+          elements[slot1.slot].key == elements[slot2.slot].key ==> slot1 == slot2
+      requires MapFromStorage(elements) == result
+      ensures forall slot :: ValidSlot(|elements|, slot) && elements[slot.slot].Entry? ==>
+          && var item := elements[slot.slot];
+          && item.key in result && result[item.key] == item.value
+      ensures forall key :: key in result ==>
+          exists slot :: ValidSlot(|elements|, slot) && elements[slot.slot] == Entry(key, result[key])
+      ensures forall key :: key !in result ==>
+          forall slot :: ValidSlot(|elements|, slot) && elements[slot.slot].Entry?
+              ==> elements[slot.slot].key != key
+    {
+      if |elements| == 0 {
+      } else if Last(elements).Entry? {
+        var item := Last(elements);
+        assert elements == DropLast(elements) + [Last(elements)];
+        var dropLastMap := MapFromStorage(DropLast(elements));
+        MapFromStorageProperties(DropLast(elements), dropLastMap);
+
+        forall slot | ValidSlot(|elements|, slot) && elements[slot.slot].Entry?
+        ensures && var item := elements[slot.slot];
+                && item.key in result && result[item.key] == item.value
+        {
+          assume false;
+        }
+        forall key | key in result
+        ensures exists slot :: ValidSlot(|elements|, slot) && elements[slot.slot] == Entry(key, result[key])
+        {
+          if key == item.key {
+            var slot := Slot(|elements| - 1);
+            assert ValidSlot(|elements|, slot);
+            assert elements[slot.slot] == Entry(key, result[key]);
+          } else {
+            assert exists slot :: ValidSlot(|elements|, slot) && elements[slot.slot] == Entry(key, result[key]);
+          }
+        }
+      } else {
+      }
+    }
+
+    predicate UnderlyingContentsMatchesContents(underlying: FixedSizeHashMap<V>)
+      reads this, underlying
+    {
+      && (forall key :: key in Contents ==> key in underlying.Contents && underlying.Contents[key] == Some(Contents[key]))
+      && (forall key :: key !in Contents ==> key !in underlying.Contents || underlying.Contents[key].None?)
+    }
+
+    predicate UnderlyingInv(underlying: FixedSizeHashMap<V>)
+    reads this, underlying, underlying.Storage
+    {
+      && |Contents| == Count as nat
+      && UnderlyingContentsMatchesContents(underlying)
+      && underlying.Inv()
+      && MapFromStorage(underlying.Storage[..]) == Contents
+    }
+
+    lemma UnderlyingInvImpliesMapFromStorageMatchesContents(underlying: FixedSizeHashMap<V>)
+      requires UnderlyingContentsMatchesContents(underlying)
+      requires underlying.Inv()
+      ensures MapFromStorage(underlying.Storage[..]) == Contents
+    {
+      // assert forall slot :: ValidSlot(underlying.Storage.Length, slot) && underlying.Storage[slot.slot].Entry? ==>
+      //     && var item := underlying.Storage[slot.slot];
+      //     && underlying.Contents[item.key] == Some(item.value);
+      // assert forall slot :: ValidSlot(underlying.Storage.Length, slot) && underlying.Storage[slot.slot].Tombstone? ==>
+      //     && var item := underlying.Storage[slot.slot];
+      //     && underlying.Contents[item.key].None?;
+      // assert forall key :: key in underlying.Contents && underlying.Contents[key].Some? ==>
+      //     exists slot :: ValidSlot(underlying.Storage.Length, slot) &&
+      //     underlying.Storage[slot.slot] == Entry(key, underlying.Contents[key].value);
+      // assert forall key :: key !in underlying.Contents || underlying.Contents[key].None? ==>
+      //     forall slot :: ValidSlot(underlying.Storage.Length, slot) && underlying.Storage[slot.slot].Entry? ==>
+      //     underlying.Storage[slot.slot].key != key;
+
+      // assert forall slot :: ValidSlot(underlying.Storage.Length, slot) && underlying.Storage[slot.slot].Entry? ==>
+      //     && var item := underlying.Storage[slot.slot];
+      //     && Contents[item.key] == item.value;
+      // assert forall slot :: ValidSlot(underlying.Storage.Length, slot) && underlying.Storage[slot.slot].Tombstone? ==>
+      //     && var item := underlying.Storage[slot.slot];
+      //     && item.key !in Contents;
+
+      // assert forall key :: key in Contents ==>
+      //     exists slot :: ValidSlot(underlying.Storage.Length, slot) &&
+      //     underlying.Storage[slot.slot] == Entry(key, Contents[key]);
+      // assert forall key :: key !in Contents ==>
+      //     forall slot :: ValidSlot(underlying.Storage.Length, slot) && underlying.Storage[slot.slot].Entry? ==>
+      //     underlying.Storage[slot.slot].key != key;
+        
+      var mapFromStorage := MapFromStorage(underlying.Storage[..]);
+      CantEquivocateMapFromStorageKey(underlying);
+      MapFromStorageProperties(underlying.Storage[..], mapFromStorage);
+      assert MapFromStorage(underlying.Storage[..]) == Contents;
+    }
+
+    predicate Inv()
+    reads this, this.Underlying, this.Underlying.Storage
+    {
+      && UnderlyingInv(Underlying)
+      && MapFromStorage(Underlying.Storage[..]) == Contents
+    }
+
+    constructor (size: uint64)
+      requires 0 < size
+      ensures Inv()
+      ensures Contents == map[]
+    {
+      Count := 0;
+      Underlying := new FixedSizeHashMap(size);
+      Contents := map[];
+
+      new;
+
+      assert forall slot :: ValidSlot(Underlying.Storage.Length, slot) ==> !Underlying.Storage[slot.slot].Entry?;
+      UnderlyingInvImpliesMapFromStorageMatchesContents(Underlying);
+      assert MapFromStorage(Underlying.Storage[..]) == Contents;
+    }
+
+    method Realloc()
+      requires Underlying.Storage.Length < 0x10000000000000000 / 2
+      requires Inv()
+      ensures Inv()
+      ensures Contents == old(Contents)
+      ensures fresh(Underlying) && fresh(Underlying.Storage)
+      modifies this
+    {
+      assert |Contents| == Count as nat;
+
+      assert 0 < Underlying.Storage.Length;
+      var newSize: uint64 := (Underlying.Storage.Length as uint64) * 2;
+      var newUnderlying: FixedSizeHashMap<V> := new FixedSizeHashMap(newSize);
+
+      assert MapFromStorage(Underlying.Storage[..]) == Contents;
+      assert MapFromStorage(newUnderlying.Storage[..]) == map[];
+
+      var i := 0;
+      ghost var transferredContents := map[];
+      while i < Underlying.Storage.Length
+        invariant i <= Underlying.Storage.Length
+        invariant newUnderlying.Inv()
+        invariant |Contents| == Count as nat
+        invariant fresh(newUnderlying) && fresh(newUnderlying.Storage)
+        invariant MapFromStorage(newUnderlying.Storage[..]) == transferredContents
+      {
+        var item := Underlying.Storage[i];
+        if item.Entry? {
+          newUnderlying.Insert(item.key, item.value);
+          transferredContents := transferredContents[item.key := item.value];
+        }
+
+        // -- increment --
+        i := i + 1;
+        // ---------------
+      }
+
+      assert |Contents| == Count as nat;
+      assert forall key :: key in Contents ==> key in newUnderlying.Contents && newUnderlying.Contents[key] == Some(Contents[key]);
+      assert forall key :: key !in Contents ==> key !in newUnderlying.Contents || newUnderlying.Contents[key].None?;
+      assert newUnderlying.Inv();
+      assert UnderlyingInv(newUnderlying);
+
+      // -- mutation --
+      Underlying := newUnderlying;
+      // --------------
+
+      assert Contents == old(Contents);
+      assert Inv();
+    }
+
+    // Insert
+    // if Underlying.Count as nat >= Underlying.Storage.Length - 1 {
+    // }
 
   }
 }
